Cleanup the correctness proof linking metarocq's pipeline with anf conversion

theories/Compiler/correctness.v
@@ -5,6 +5,7 @@ Require Export LambdaANF.toplevel Codegen.toplevel CodegenWasm.toplevel.
 Require Import LambdaBox_to_LambdaANF.fuel_sem.
 Require Import LambdaBox_to_LambdaANF.common.
 Require Import LambdaBox_to_LambdaANF.anf.
+Require Import LambdaBox_to_LambdaANF.anf_correct.
 Require Import LambdaBox_to_LambdaANF.anf_toplevel.
 Require Export LambdaANF.toplevel_theorems.
 Require Import compcert.lib.Maps.
@@ -26,95 +27,111 @@ Import MonadNotation.
 Import ListNotations.
 Import common rel_comp.
 Require Import LambdaANF.term.
-Print CertiRocq_pipeline.
-Print get_options.
-Print compile_LambdaBoxEAst.
-Print erase_program.
-Print compile_LambdaANF_ANF.
 
 Definition next_id := 100%positive.
 Definition econf := Erasure.default_erasure_config.
-Definition opts := default_opts.
-
-Definition run_pipeline p pre :=
-  let p' := Transform.Transform.run (verified_lambdabox_pipeline econf) p pre in
-  let (perr, log) := run_pipeline _ _ opts p' (compile_LambdaANF_ANF next_id []) in
-  match perr with
-  | Ret p =>
-    let '(pr, cenv, _, _, nenv, fenv, idm,  e) := p in
-    Some (nenv, cenv, idm, e)
-  | Err s => None
-  end.
 Import EEnvMap.
 
 From MetaRocq.Erasure Require Import EWcbvEval.
-Section lambdabox_anf_pipeline_correct.
 Import EGlobalEnv.
+Import ETransform EImplementLazyForce EImplementBox.
+
+Definition env_flags :=
+  let efl := EConstructorsAsBlocks.switch_cstr_as_blocks
+    (EInlineProjections.disable_projections_env_flag 
+      (ERemoveParams.switch_no_params EWellformed.all_env_flags)) in
+  let efl' := efl_coind_to_ind efl in
+  switch_off_thunk (switch_off_box efl').
+
+(* CertiRocq does not support primitives yet *)
+Definition no_primitive_flags := {|
+  has_primint := false;
+  has_primfloat := false;
+  has_primstring := false;
+  has_primarray := false; |}.
+  
+Definition switch_off_primitives (fl : ETermFlags) :=
+{| has_tBox := fl.(has_tBox)
+  ; has_tRel := fl.(has_tRel)
+  ; has_tVar := fl.(has_tVar)
+  ; has_tEvar := fl.(has_tEvar)
+  ; has_tLambda := fl.(has_tLambda)
+  ; has_tLetIn := fl.(has_tLetIn)
+  ; has_tApp := fl.(has_tApp)
+  ; has_tConst := fl.(has_tConst)
+  ; has_tConstruct := fl.(has_tConstruct)
+  ; has_tCase := fl.(has_tCase)
+  ; has_tProj := fl.(has_tProj)
+  ; has_tFix := fl.(has_tFix)
+  ; has_tCoFix := fl.(has_tCoFix)
+  ; has_tPrim := no_primitive_flags
+  ; has_tLazy_Force := fl.(has_tLazy_Force)
+|}.
+
+(* CertiRocq's correctness lemma only supports global environments made of lambda abstractions 
+  (not arbitrary expressions or values) *)
+Lemma lambda_glob_lookup Σ :
+  lambda_glob Σ -> 
+  forall kn v, EGlobalEnv.lookup_env Σ kn = Some (ConstantDecl {| cst_body := Some v |}) -> 
+  lambda_value_pred Σ v.
+Proof.
+  induction 1.
+  - intros kn v; cbn => //.
+  - intros kn' v' hl. 
+    cbn in hl. 
+    destruct (eqb_specT kn' kn). subst kn'. noconf hl.
+    destruct d0 as [na [t ->]]. now do 2 eexists.
+    now cbn in d0.
+Qed.
+
+Lemma lambda_glob_declared Σ {efl : EEnvFlags} : 
+  wf_glob Σ ->
+  EWcbvEval.lambda_glob Σ ->
+  forall (k : kername) (decl : constant_body),
+  declared_constant Σ k decl ->
+  decl_pred (lambda_value_pred Σ) (ConstantDecl decl).
+Proof.
+  unfold EGlobalEnv.declared_constant.
+  intros hwf hv kn decl hl. destruct decl as [] => //.
+  destruct cst_body => //.
+  eapply lambda_glob_lookup in hl; tea.
+Qed.
+
+(* If the global environment is made of lambdas the all entries evaluate in 0 steps into values *)
+Lemma lambda_glob_eval_env_fuel (p : EProgram.eprogram) (efl := env_flags) :
+  wf_glob p.1 ->
+  EWcbvEval.lambda_glob p.1 ->
+  forall (k : kername) (decl : constant_body) (body : term),
+  EGlobalEnv.declared_constant p.1 k decl ->
+  cst_body decl = Some body -> exists (src_v : fuel_sem.value) (f t : nat), 
+  eval_env_fuel (Hf:=LambdaBox_resource_fuel) p.1 [] body (Val src_v) f t /\ f = <0>.
+Proof.
+  destruct p as [Σ p]; cbn; clear p.
+  intros hwf hv kn decl body hd hb.
+  have hwfd := wf.wf_glob_globals_wf _ hwf _ _ _ hd hb.
+  eapply (lambda_glob_declared _ hwf hv) in hd; tea.
+  destruct decl as [[|]]=> //. noconf hb. cbn in hd.
+  destruct hd as [na [b ->]]. do 3 eexists. split. constructor. constructor. now cbn.
+Qed.
 
 Section Assumptions.
 
-  Lemma lambda_glob_lookup Σ : 
-    lambda_glob Σ -> 
-    forall kn v, EGlobalEnv.lookup_env Σ kn = Some (ConstantDecl {| cst_body := Some v |}) -> 
-    lambda_value_pred Σ v.
-  Proof.
-    induction 1.
-    - intros kn v; cbn => //.
-    - intros kn' v' hl. 
-      cbn in hl. 
-      destruct (eqb_specT kn' kn). subst kn'. noconf hl.
-      destruct d0 as [na [t ->]]. now do 2 eexists.
-      now cbn in d0.
-  Qed.
-
-  Lemma lambda_glob_declared Σ {efl : EEnvFlags} : 
-    wf_glob Σ ->
-    EWcbvEval.lambda_glob Σ ->
-    forall (k : kername) (decl : constant_body),
-    declared_constant Σ k decl ->
-    decl_pred (lambda_value_pred Σ) (ConstantDecl decl).
-  Proof.
-    unfold EGlobalEnv.declared_constant.
-    intros hwf hv kn decl hl. destruct decl as [] => //.
-    destruct cst_body => //.
-    eapply lambda_glob_lookup in hl; tea.
-  Qed.
-  Import ETransform EImplementLazyForce EImplementBox.
-  
-  Definition env_flags :=
-     let efl := EConstructorsAsBlocks.switch_cstr_as_blocks
-        (EInlineProjections.disable_projections_env_flag 
-          (ERemoveParams.switch_no_params EWellformed.all_env_flags)) in
-     let efl' := efl_coind_to_ind efl in
-     switch_off_thunk (switch_off_box efl').
-
-  Definition no_primitive_flags := {|
-    has_primint := false;
-    has_primfloat := false;
-    has_primstring := false;
-    has_primarray := false; |}.
-
-  Lemma lambda_glob_eval_env_fuel (p : EProgram.eprogram) (efl := env_flags) :
-    wf_glob p.1 ->
-    EWcbvEval.lambda_glob p.1 ->
-    forall (k : kername) (decl : constant_body) (body : term),
-    EGlobalEnv.declared_constant p.1 k decl ->
-    cst_body decl = Some body -> exists (src_v : fuel_sem.value) (f t : nat), 
-    eval_env_fuel (Hf:=anf_correct.LambdaBox_resource_fuel) p.1 [] body (Val src_v) f t /\ f = <0>.
-  Proof.
-    destruct p as [Σ p]; cbn; clear p.
-    intros hwf hv kn decl body hd hb.
-    have hwfd := wf.wf_glob_globals_wf _ hwf _ _ _ hd hb.
-    eapply (lambda_glob_declared _ hwf hv) in hd; tea.
-    destruct decl as [[|]]=> //. noconf hb. cbn in hd.
-    destruct hd as [na [b ->]]. do 3 eexists. split. constructor. constructor. now cbn.
-  Qed.
-
   Context (func_tag kon_tag default_tag default_itag : positive)
           (tgm : conId_map).
+  (* The conId_map must be injective *)          
+  Context (Htgm : forall dc dc' : dcon, dcon_to_tag default_tag dc tgm = dcon_to_tag default_tag dc' tgm -> dc = dc').
+  
+  (* This property should come from the well-formedness of terms w.r.t. their global environment, 
+    currently missing in the ANF proof. 
+    The list of [ctor_tag × exp] is built from the [ind] annotation of the Case construct in the anf, 
+    and these lemma is used where [ctag] is built from [ind] as well. *)
+  Context (casecon : forall p : EProgram.eprogram, 
+    let ie := inductive_env_east (fst p) in
+    forall (P : list (ctor_tag × exp)) (ctag : ctor_tag), 
+    term_util.caseConsistent (top_cenv default_tag default_itag ie) 
+      P ctag).
 
   Notation refines_top Σ := (@refines_top default_tag default_itag tgm Σ).
-
 
   (** To prove the correctness of connecting the MetaRocq pipeline and CertiRocq's ANF, we
       need a stronger well-formedness property. This formalizes the remaining mismatch 
@@ -123,44 +140,28 @@ Section Assumptions.
     - primitives are not supported in fuel_sem, and primitive arrays are forbidden in ANF conversion.
     - the environment must be axiom free, as usual *)
 
-  Definition switch_off_primitives (fl : ETermFlags) :=
-  {| has_tBox := fl.(has_tBox)
-    ; has_tRel := fl.(has_tRel)
-    ; has_tVar := fl.(has_tVar)
-    ; has_tEvar := fl.(has_tEvar)
-    ; has_tLambda := fl.(has_tLambda)
-    ; has_tLetIn := fl.(has_tLetIn)
-    ; has_tApp := fl.(has_tApp)
-    ; has_tConst := fl.(has_tConst)
-    ; has_tConstruct := fl.(has_tConstruct)
-    ; has_tCase := fl.(has_tCase)
-    ; has_tProj := fl.(has_tProj)
-    ; has_tFix := fl.(has_tFix)
-    ; has_tCoFix := fl.(has_tCoFix)
-    ; has_tPrim := no_primitive_flags
-    ; has_tLazy_Force := fl.(has_tLazy_Force)
-  |}.
-  
+
   Definition certirocq_flags (efl : EEnvFlags) := 
     {| has_axioms := false; 
        has_cstr_params := efl.(has_cstr_params); 
-       term_switches := switch_off_primitives efl.(term_switches);
+       term_switches := disable_box_term_flags (switch_off_primitives efl.(term_switches));
        cstr_as_blocks := efl.(cstr_as_blocks) |}.
 
+  Definition anf_convert := 
+    convert_top_anf func_tag default_tag (M.empty _) default_itag next_id tgm []
+      (fun _ => None).
+  
   Theorem correctness_from_erasure (p : EProgram.eprogram) : 
     (* The postcondition on MetaRocq's pipeline *)
     Transform.Transform.post (certirocq_post_metarocq_pipeline econf) p ->
     (* Stronger invariant: no axioms, no primitives *)
-    EProgram.wf_eprogram (certirocq_flags (switch_off_box env_flags)) p ->
+    EProgram.wf_eprogram (certirocq_flags env_flags) p ->
     let ie := inductive_env_east (fst p) in
-    forall (casecon : forall (P : list (ctor_tag × exp)) (ctag : ctor_tag), term_util.caseConsistent (top_cenv default_tag default_itag ie) P ctag),
-    forall e_tgt comp_d',  
-      convert_top_anf func_tag default_tag (M.empty _) default_itag next_id tgm []
-      (fun _ => None)
-      ie (List.rev (fst p)) (snd p) = (compM.Ret e_tgt, comp_d') ->
-    exists M, refines_top (fst p) ie M (snd p) e_tgt.
+    forall e_tgt comp_d', 
+      anf_convert ie (List.rev (fst p)) (snd p) = (compM.Ret e_tgt, comp_d') ->
+      exists M, refines_top (fst p) ie M (snd p) e_tgt.
   Proof.
-    intros hp wf' ie case_con e_tgt comp_d' cvt.
+    intros hp wf' ie e_tgt comp_d' cvt.
     cbn in hp.
     match goal with
     | [ _ : EProgram.wf_eprogram ?fl p /\ _ |- _ ] => set (efl := fl) in *
@@ -168,8 +169,6 @@ Section Assumptions.
     destruct hp as [wfp [vg]].
     eapply (convert_top_anf_correct func_tag kon_tag default_tag default_itag tgm (fst p) 
       (efl:=certirocq_flags (switch_off_box env_flags))); trea.
-    - (* If tgm came from convert_env, wouldn't that be true? *)
-      admit.
     - (* The environment entries evaluate to values *)
       intros kn decl hl hb hbody.
       eapply lambda_glob_eval_env_fuel in hb; tea.
@@ -183,85 +182,14 @@ Section Assumptions.
     - (* Wellformed declarations in the global environment *) 
       clear wfp. destruct wf' as [wfΣ wf].       
       intros kn decl body hdecl hb.
-      Set Printing All.
       eapply (lookup_env_wellformed (efl := certirocq_flags (switch_off_box env_flags))) in hdecl; tea.
       destruct decl; trivial. cbn in hdecl. cbn in hb.
       now subst cst_body.
     - apply wf'.
     - (* No prims *)
       intros s. cbn. reflexivity.
+    - apply casecon.
     - apply wf'.
   Qed.
 
-(*
-Section Assumptions.
-  
-  Context (func_tag kon_tag default_tag default_itag : positive)
-          (tgm : conId_map).
-
-  Context (box_dc : dcon)
-          (box_tag : dcon_to_tag default_tag tgm = default_tag).
-
-  Let Hf_src := LambdaBox_resource_fuel default_tag tgm box_tag.
-  Let Ht_src := LambdaBox_resource_trace default_tag tgm box_tag.
-  
-  Existing Instance default_wcbv_flags. 
-
-  Context {fuel trace : Type}.
-  Context {Hf : @fuel_resource fuel} {Ht : @trace_resource trace}.
-Transparent bind.
-Transparent Pipeline_utils.ret.
-
-
-
-
-  Theorem correctness_from_erasure (p : EProgram.eprogram_env) : 
-  forall pre : Transform.Transform.pre (verified_lambdabox_pipeline econf) p,
-  forall v, 
-    EWcbvEval.eval (GlobalContextMap.global_decls (fst p)) (snd p) v ->
-    exists nenv cenv cm e ev v' n r fuel trace, 
-      run_pipeline p pre = Some (nenv, cenv, e) /\
-      @eval_env_step _ Hf_src Ht_src [] [] v (Val v') n r /\
-      eval.bstep_fuel (Hf:=Hf) (Ht := Ht) (snd nenv) emp e fuel (eval.Res ev) trace /\
-      anf_util.anf_val_rel (Hf_src := Hf_src) (Ht_src:=Ht_src) func_tag default_tag tgm cm (fst p) v' ev.
-  Proof.
-    intros pre v ev.
-    unfold run_pipeline.
-    unfold Pipeline_utils.run_pipeline, runState.
-    unfold Transform.Transform.run, Transform.time.
-    set (tr := Transform.Transform.transform _ _ _).
-    unfold compile_LambdaANF_ANF. unfold debug_msg, get_options, compM.ask. unfold opts, default_opts.
-    About bind.
-    cbn -[tr].
-    destruct (LambdaANF_ANF _ _ _ ) eqn:ela.
-    unfold LambdaANF_ANF in ela.
-    Search anf.convert_top_anf. 
-
-
-    { exfalso.
-      unfold LambdaANF
-    
-    }
-    cbn. destruct get_options. cbn. 
-    Set Printing All. unfold tmBind. cbn.
-
-
-
-
-
-
-From MetaRocq.Template Require Import WcbvEval TemplateProgram.
-
-Theorem correctness mapping (p : template_program) : 
-  Transform.Transform.pre (erasure_pipeline_mapping econf) (mapping, p) ->
-  forall v, 
-    eval (fst p) (snd p) v ->
-    exists nenv cenv fuel trace e v' n r, 
-      run_pipeline p = Some (nenv, cenv, e) /\ 
-      eval.bstep_fuel cenv emp e fuel (eval.Res v1) trace /\
-      eval_env_step [] v v' n r.
-
-
-
-
-*)
+End Assumptions.
